$$

    Q(w) = \dfrac{1}{\ell} \left( y - Xw \right)^T \left( y - Xw \right)

$$

$$
\begin{align}
dQ(w) = \frac{1}{l}d\left[   (y-Xw)^{T}\right(y-Xw)] =  \\
= \frac{1}{l}\left[ d(y-Xw)^{T}(y-Xw)+ (y-Xw)^{T}d(y-Xw) \right] = \\
= \frac{1}{l}\left[ d(y^{T}-w^{T}X^{T})(y-Xw)+ (y-Xw)^{T}(\cancelto{ 0 }{ dy }-dXw) \right] = \\
= \frac{1}{l}\left[ (\cancelto{ 0 }{ dy^{T} }-dw^{T}X^{T})(y-Xw)+ (y-Xw)^{T}(-\cancelto{ 0 }{ dX }w) \right] = \\
= {1}/{l}\left[ (-dw^{T}X^{T})(y-Xw) \right] = \frac{1}{l}(-dw^{T}X^{T}y + \underbrace{ dw^{T}X^{T}Xw }_{ scalar }) =  \\
= {1}/{l}(-y^{T}Xdw + w^{T}X^{T}Xdw) = \frac{1}{l}(w^{T}X^{T} - y&^{T})Xdw
\end{align}
$$