![[Pasted image 20240204205854.png]]
a)
$$
\begin{align}
b_{t} = t^{2} + 6t + u_{t} - 4Lu_{t} - 4L^{2}u_{t} \implies   \\
b_{t} = t^{2} + 6t + u_{t} - 4u_{t-1} - 4u_{t-2}
\end{align}
$$
b) 
$$
\begin{align}
E(b_{t}) = E\left[ t^{2} + 6t + u_{t} - 4u_{t-1} - 4u_{t-2} \right] = \\
= E\left[ t^{2} \right] + 6E[t] - \cancelto{ 0, \text{White Noise} }{ 4E[u_{t-1}] } + \cancelto{ 0 }{ E[u_{t}] } - \cancelto{ 0 }{ 4E[u_{t-2}] }  
= t^{2} + 6t  \\ \\
Var(b_{t}) = Var\left[ t^{2} + 6t + u_{t} - 4u_{t-1} - 4u_{t-2} \right] =  \\
= Var\left[u_{t} - 4u_{t-1} - 4u_{t-2} \right] = \{ Cov(u_t,u_{s})=0 \} = \\
= Var[u_{t}] + 16Var[u_{t-1}] + 16Var[u_{t-2}] = 33\sigma^{2}
\end{align}

$$
—Å) 
$$
\begin{align}
&Cov(b_{t}, b_{t-k}) = Cov\Big(t^{2} + 6t + u_{t} - 4u_{t-1} - 4u_{t-2}; \quad  (t-k)^{2} + 6(t-k) + u_{(t-k)} - 4u_{t-k-1} - 4u_{t-k-2}\Big)= \\
&= Cov(u_{t} - 4u_{t-1}-4u_{t-2};\; u_{t-k} -4u_{t-k-1} - 4u_{t-k-2}) =  \\
&= \cancelto{ 0 }{ Cov(u_{t}, u_{t-k}) } - \cancelto{ 0 }{ 4Cov(u_{t}, u_{t-k-1}) } - \dots +\cancelto{ 0 }{ 16Cov(u_{t-2}, u_{t-k-2}) } =  \\
&= \text{By white noise def.} = 0
\end{align}
$$
